Add documentation to example

src/examples/hello_liveness.v
@@ -2,6 +2,12 @@ From TLA Require Import logic.
 
 Section example.
 
+(*|
+We define a simple state machine with a field `x` that goes from `A` to `B` to `C`, and separately a field `happy` that remains constant.
+
+The state machine has a safety property that says `happy` is true, and a liveness property that eventually `x = C`.
+|*)
+
 Inductive abc := A | B | C.
 Record state :=
   { x: abc; happy: bool; }.
@@ -14,11 +20,19 @@ Definition ab : action state :=
 Definition bc : action state :=
   λ s s', (s.(x) = B ∧ s'.(x) = C ∧ s'.(happy) = s.(happy)).
 
+Definition init (s: state) :=
+    s.(x) = A ∧ s.(happy) = true.
+
+(*|
+It is important to allow stuttering (`s = s'`) in this predicate! Otherwise there would be no infinite sequences satisfying `□ ⟨next⟩`, since after two transitions no steps would be possible.
+|*)
 Definition next s s' :=
   ab s s' ∨ bc s s' ∨ s = s'.
 
-Definition init (s: state) : Prop := s.(x) = A ∧ s.(happy).
 
+(*|
+A little automation will prove all the state-machine specific reasoning required for this example, essentially by brute force.
+|*)
 Hint Unfold init happy next ab bc : stm.
 
 Ltac stm :=
@@ -38,15 +52,33 @@ Ltac stm :=
       end;
     intuition (subst; eauto; try congruence) ].
 
+(*|
+--------
+Safety
+--------
+
+The safety property is pretty easy, using `init_invariant`. In fact it's so simple it's already inductive and we don't need to go through a separate invariant.
+|*)
+
 Theorem always_happy :
   state_pred init ∧ □ ⟨next⟩ ⊢ □ (state_pred (λ s, s.(happy))).
 Proof.
-  apply (init_safety _ _ (state_pred (λ s, s.(happy))) _).
-  - apply state_pred_impl => s.  stm.
-  - apply action_preserves_inv => s s'.  stm.
-  - reflexivity.
+  apply init_invariant.
+  - stm.
+  - stm.
 Qed.
 
+(*|
+-----------
+Liveness
+-----------
+
+Liveness is more interesting. The high-level strategy is to use the rule `wf1` to prove A ~~> B and that B ~~> C; then we can chain them together and finally apply them by showing that `init` implies A.
+|*)
+
+(*|
+Notice that the state-machine reasoning all happens here, and in the analogous `b_leads_to_c` proof below. We only need to prove one- and two-state properties and the wf1 rules lifts them to a temporal property that uses the weak fairness assumption.
+|*)
 Theorem a_leads_to_b :
   □ ⟨ next ⟩ ∧ weak_fairness ab ⊢
   state_pred (λ s, s.(x) = A) ~~> state_pred (λ s, s.(x) = B).
@@ -63,6 +95,9 @@ Proof.
   apply state_pred_impl => s.  stm.
 Qed.
 
+(*|
+This theorem isn't directly needed; we carry out the same reasoning to derive ◇ C from the leads_to proofs.
+|*)
 Theorem eventually_b :
   state_pred init ∧ □ ⟨next⟩ ∧ weak_fairness ab ⊢
   ◇ (state_pred (λ s, s.(x) = B)).
